optimizations.v
@@ -2,6 +2,7 @@ Require Import Arith.
 Require Import Nat.
 Require Import Bool.
 Require Import bbv.Word.
+Require Import Coq.NArith.NArith.
 Require Import List.
 Require Import Coq_EVM.definitions.
 Import EVM_Def Concrete Abstract Optimizations.
@@ -915,6 +916,9 @@ Proof.
 apply optimize_fresh_var_preservation.
 apply optimize_add_zero_fvar_safe.
 Qed.
+
+
+
 
 
 (****************************************** 
@@ -2049,6 +2053,73 @@ match map with
                       end
 end.
 
+Lemma gt_iszero_nat: forall (x: nat),
+x <? 1 = true <-> x = 0.
+Proof.
+split.
+- intros. destruct x as [|x'].
+  + reflexivity.
+  + simpl in H. unfold ltb in H. simpl in H. discriminate.
+- intros. rewrite -> H. auto.
+Qed.
+
+Search(_ <> _).
+Lemma gt_iszero_nat': forall (x: nat),
+x <? 1 = false <-> x <> 0.
+Proof.
+split.
+- intros. destruct x as [|x'].
+  + unfold ltb in H. rewrite -> Nat.leb_refl in H. discriminate.
+  + auto.
+- intros. destruct x as [|x']. 
+  + unfold not in H. exfalso. auto.
+  + unfold ltb. simpl. reflexivity.
+Qed.
+
+Search (N.to_nat).
+Lemma gt_N_nat: forall (x y: N) (b: bool),
+(x <? y)%N = b -> (N.to_nat x) <? (N.to_nat y) = b.
+Proof.
+Admitted.
+
+Check Logic.not.
+Lemma word_eq_zero: forall (x: EVMWord),
+N.to_nat (wordToN x) = 0 -> x = WZero.
+Proof.
+intros. destruct (weqb x WZero) eqn: eq_x_wzero.
+- apply weqb_sound. assumption.
+- apply weqb_false in eq_x_wzero.
+  admit.
+Admitted.
+
+Lemma word_neq_zero: forall (x: EVMWord),
+N.to_nat (wordToN x) <> 0 -> x <> WZero.
+Proof.
+intros. destruct (weqb x WZero) eqn: eq_x_wzero.
+- apply weqb_sound in eq_x_wzero. rewrite eq_x_wzero in H.
+  simpl in H. auto.
+- apply weqb_false. assumption.
+Qed.
+
+Lemma Ntonat_1: (N.to_nat 1)%N = S 0.
+Proof. auto. Qed.
+
+Search (weqb).
+Lemma gt_iszero: forall (x: EVMWord),
+evmgt [WOne; x] = iszero [x].
+Proof.
+intros. simpl. destruct ((wordToN x <? 1)%N) eqn: oneN.
+- apply gt_N_nat in oneN. rewrite -> Ntonat_1 in oneN.
+  apply gt_iszero_nat in oneN. 
+  apply word_eq_zero in oneN. rewrite oneN.
+  rewrite -> weqb_reflex. reflexivity.
+- apply gt_N_nat in oneN. rewrite -> Ntonat_1 in oneN.
+  apply gt_iszero_nat' in oneN. 
+  pose proof (word_neq_zero x oneN).
+  apply weqb_ne in H. rewrite -> H.
+  reflexivity.
+Qed.
+
 Definition optimize_gt_one_fvar (fresh_var: nat) (s: asfs) : option asfs :=
 optimize_func_map optimize_map_gt_one fresh_var s.
 
@@ -2056,10 +2127,161 @@ optimize_func_map optimize_map_gt_one fresh_var s.
 Definition optimize_gt_one (a: asfs) : asfs*bool :=
 optimize_fresh_var optimize_gt_one_fvar a.
 
+Lemma eq_eval_opt_gt_one: forall (m1 m2: asfs_map) (ops: opm) (n: nat)
+  (stack: tstack),
+ops GT = Some (Op false 2 evmgt) ->
+ops ISZERO = Some (Op false 1 iszero) ->
+optimize_map_gt_one n m1 = Some m2 ->
+forall (elem: asfs_stack_val), eval_asfs2_elem stack elem m1 ops =
+                               eval_asfs2_elem stack elem m2 ops.
+Proof.
+induction m1 as [|h t IH].
+- intros. simpl in H1. discriminate.
+- intros. simpl in H1. destruct h as [hn hv] eqn: eq_h.
+  destruct (hn =? n) eqn: eq_hn_n.
+  + (* We have found the fresh variable to optimize in the map *) 
+    destruct (hv) as [basicval|opval] eqn: eq_hv; try discriminate.
+    destruct (opval) eqn: eq_opval; try discriminate.
+    destruct args as [| arg1 ta]; try discriminate.
+    destruct ta as [| arg2 tta]; try discriminate.
+    destruct tta; try discriminate.
+    destruct (stack_val_has_value' arg1 t WOne ) eqn: eq_arg1_one;
+      try discriminate.
+    injection H1 as eq_m2. rewrite <- eq_m2.
+    destruct elem as [val|var|fvar] eqn: eq_elem.
+    * apply eval_asfs2_val.
+    * apply eval_var.
+    * unfold eval_asfs2_elem. destruct (hn =? fvar) eqn: eq_vame_fvar.
+      -- rewrite -> H. simpl. fold eval_asfs2_elem.
+         rewrite -> stack_val_has_value_eval' with (v:=WOne);
+           try assumption.
+         rewrite -> H0.
+         destruct (eval_asfs2_elem stack arg2 t ops) as [arg2_val|]
+           eqn: eq_eval_arg2; try reflexivity.
+         apply gt_iszero.
+      -- fold eval_asfs2_elem. reflexivity.
+  + (* This is not yet the fresh variable to optimize*) 
+    destruct (optimize_map_gt_one n t) as [map'|] eqn: eq_optimize_t; 
+      try discriminate.
+    injection H1 as H1. rewrite <- H1. 
+    destruct elem as [val|var|fvar] eqn: eq_elem; try reflexivity.
+    simpl. destruct (hn =? fvar) eqn: eq_hn_fvar.
+    * destruct hv eqn: eq_hv.
+      -- apply IH with (n:=n); try assumption.
+      -- rewrite -> eval_asfs2_ho. rewrite -> eval_asfs2_ho.
+         pose proof (IH map' ops n stack H H0 eq_optimize_t) as IHc.
+         pose proof (eq_eval_elem_stack stack t map' ops args IHc) as
+           eq_eval_t_map'.
+         rewrite -> eq_eval_t_map'. reflexivity.
+    * apply IH with (n:=n); try assumption.
+Qed.
+
+Theorem optimize_gt_one_fvar_eq: forall (a1 a2: asfs) (fresh_var: nat)
+  (c: tstack) (ops: opm),
+ops GT = Some (Op false 2 evmgt) ->
+ops ISZERO = Some (Op false 1 iszero) ->
+optimize_gt_one_fvar fresh_var a1 = Some a2 ->
+eval_asfs c a1 ops = eval_asfs c a2 ops.
+Proof.
+intros.
+destruct a1 as [h1 maxid1 s1 m1] eqn: eq_a1.
+destruct a2 as [h2 maxid2 s2 m2] eqn: eq_a2.
+simpl in H1.
+destruct (optimize_map_gt_one fresh_var m1) eqn: eq_opt_map;
+  try discriminate.
+injection H1 as Hh1h2 Hmaxid1_2 Hs1s2 Hm1a.
+rewrite -> Hm1a in eq_opt_map.
+pose proof (eq_eval_opt_gt_one m1 m2 ops fresh_var c H H0 eq_opt_map)
+  as Hall_elem_eval_same_m1_m2.
+simpl. rewrite -> Hh1h2. rewrite -> Hs1s2.
+destruct (length c =? h2); try reflexivity.
+apply eq_eval_elem_stack. assumption.
+Qed.
+
+
+Lemma opt_gt_one_same_fvar_in_maps: forall (n: nat)
+  (m1 m2: asfs_map),
+optimize_map_gt_one n m1 = Some m2 ->
+same_fvar_in_maps m1 m2.
+Proof.
+intros n m1. revert n.
+induction m1 as [| h t IH].
+- intros n m2 Hopt. simpl in Hopt. discriminate.
+- intros n m2 Hopt.
+  simpl in Hopt.
+  destruct h as [fvar efvar] eqn: eq_h.
+  destruct (fvar =? n) eqn: eq_fvar_n.
+  + destruct efvar eqn: eq_efvar; try discriminate.
+    destruct opcode eqn: eq_opcode; try discriminate.
+    destruct args as [| arg1 targs1] eqn: eq_args; try discriminate.
+    destruct targs1 as [| arg2 targs2] eqn: eq_args1; try discriminate.
+    destruct targs2 eqn: eq_args2; try discriminate.
+    destruct (stack_val_has_value' arg1 t WOne); try discriminate.
+    injection Hopt as eq_m2. rewrite <- eq_m2.
+    simpl. split; try reflexivity.
+    apply same_fvar_refl.
+  + destruct (optimize_map_gt_one n t) as [t_opt|] eqn: optimize_t;
+      try discriminate.
+    pose proof (strictly_decreasing_preserv fvar efvar t) 
+      as Hdecr_t.
+    pose proof (IH n t_opt optimize_t).
+    simpl. injection Hopt as eq_m2. rewrite <- eq_m2.
+    split; try reflexivity. assumption.
+Qed.
+
+
+Lemma opt_gt_one_decreasingness_preservation: forall (n: nat)
+  (m1 m2: asfs_map),
+strictly_decreasing_map m1 ->
+optimize_map_gt_one n m1 = Some m2 ->
+strictly_decreasing_map m2.
+Proof.
+intros.
+apply opt_gt_one_same_fvar_in_maps in H0.
+apply same_fvar_in_map_preserves_decreasingness with (m1:=m1);
+  try assumption.
+Qed.
+
+
+Lemma optimize_gt_one_fvar_safe:
+safe_optimization_fvar optimize_gt_one_fvar.
+Proof.
+unfold safe_optimization_fvar. intros.
+split.
+- assert (opmap GT = Some (Op false 2 evmgt)) as Hopmap; try reflexivity.
+  assert (opmap ISZERO = Some (Op false 1 iszero)) as Hopmap'; try reflexivity.
+  pose proof (optimize_gt_one_fvar_eq a opt_a n c opmap Hopmap Hopmap' H0)
+    as Heq_eval_a_opta.
+  rewrite -> Heq_eval_a_opta in H.
+  rewrite -> H.
+  split; try reflexivity.
+- unfold valid_asfs.
+  destruct opt_a as [hopt maxopt sopt mopt] eqn: eq_opt_a.
+  destruct a as [ha maxa sa ma] eqn: eq_a.
+  simpl in H1. simpl in H0.
+  destruct (optimize_map_gt_one n ma) eqn: optimize_ma; try discriminate.
+  injection H0 as eq_h eq_max eq_stack eq_maps. 
+  rewrite -> eq_maps in optimize_ma.
+  destruct H1 as [Hfreshv Hdecr].
+  rewrite <- eq_max.
+  rewrite <- eq_maps.
+  split.
+  + apply same_fvar_in_map_preserves_fresh_var_gt with (m1:=ma).
+    * assumption.
+    * apply opt_gt_one_same_fvar_in_maps with (n:=n).
+      rewrite -> eq_maps. assumption.
+  + apply opt_gt_one_decreasingness_preservation with (n:=n) (m1:=ma) 
+      (m2:=a0) in Hdecr.
+    * assumption.
+    * rewrite -> eq_maps. assumption.
+Qed.
+
 Theorem optimize_gt_one_safe:
 safe_optimization optimize_gt_one.
 Proof.
-Admitted.
+apply optimize_fresh_var_preservation.
+apply optimize_gt_one_fvar_safe. 
+Qed.
 
 
 
@@ -2122,17 +2344,197 @@ match map with
                       end
 end.
 
+Search (wor).
+Lemma or_comm: forall (x y: EVMWord),
+or [x;y] = or [y;x].
+Proof.
+intros. unfold or. rewrite -> wor_comm. reflexivity.
+Qed.
+
+Lemma or_zero: forall (x: EVMWord),
+or [x;WZero] = Some x.
+Proof.
+intros. rewrite or_comm. unfold or. rewrite -> wor_wzero. reflexivity.
+Qed.
+
+
 Definition optimize_or_zero_fvar (fresh_var: nat) (s: asfs) : option asfs :=
 optimize_func_map optimize_map_or_zero fresh_var s.
 
-(* This is the main optimization *)
 Definition optimize_or_zero (a: asfs) : asfs*bool :=
 optimize_fresh_var optimize_or_zero_fvar a.
+
+Lemma eq_eval_opt_or_zero: forall (m1 m2: asfs_map) (ops: opm) (n: nat)
+  (stack: tstack),
+ops OR = Some (Op true 2 or) ->
+optimize_map_or_zero n m1 = Some m2 ->
+forall (elem: asfs_stack_val), eval_asfs2_elem stack elem m1 ops =
+                               eval_asfs2_elem stack elem m2 ops.
+Proof.
+induction m1 as [|h t IH].
+- intros. simpl in H0. discriminate.
+- intros. simpl in H0. destruct h as [hn hv] eqn: eq_h.
+  destruct (hn =? n) eqn: eq_hn_n.
+  + (* We have found the fresh variable to optimize in the map *) 
+    destruct (hv) as [basicval|opval] eqn: eq_hv; try discriminate.
+    destruct (opval) eqn: eq_opval; try discriminate.
+    destruct args as [| arg1 ta]; try discriminate.
+    destruct ta as [| arg2 tta]; try discriminate.
+    destruct tta; try discriminate.
+    destruct (stack_val_has_value' arg1 t WZero ) eqn: eq_arg1_zero.
+    * (* arg1 is WZero *)
+      injection H0 as eq_m2. rewrite <- eq_m2.
+      destruct elem as [val|var|fvar] eqn: eq_elem.
+      -- apply eval_asfs2_val.
+      -- apply eval_var.
+      -- unfold eval_asfs2_elem. destruct (hn =? fvar) eqn: eq_vame_fvar.
+         ++ rewrite -> H. simpl. fold eval_asfs2_elem.
+            rewrite -> stack_val_has_value_eval' with (v:=WZero);
+              try assumption.
+            destruct (eval_asfs2_elem stack arg2 t ops) as [arg2_val|]
+              eqn: eq_eval_arg2; try reflexivity.
+            rewrite -> or_comm. rewrite -> or_zero. reflexivity.
+         ++ fold eval_asfs2_elem. reflexivity.
+    * (* arg2 is WZero *)
+      destruct (stack_val_has_value' arg2 t WZero) eqn: eq_arg2_zero;
+        try discriminate.
+      injection H0 as eq_m2. rewrite <- eq_m2.
+      destruct elem as [val|var|fvar] eqn: eq_elem.
+      -- apply eval_asfs2_val.
+      -- apply eval_var.
+      -- unfold eval_asfs2_elem. destruct (hn =? fvar) eqn: eq_vame_fvar.
+         ++ rewrite -> H. simpl. fold eval_asfs2_elem.
+            destruct (eval_asfs2_elem stack arg1 t ops) as [arg1_val|]
+              eqn: eq_eval_arg2; try reflexivity.
+            rewrite -> stack_val_has_value_eval' with (v:=WZero);
+              try assumption.
+            rewrite -> or_zero. reflexivity. 
+         ++ fold eval_asfs2_elem. reflexivity.
+  + (* This is not yet the fresh variable to optimize*) 
+    destruct (optimize_map_or_zero n t) as [map'|] eqn: eq_optimize_t; 
+      try discriminate.
+    injection H0 as H0. rewrite <- H0. 
+    destruct elem as [val|var|fvar] eqn: eq_elem; try reflexivity.
+    simpl. destruct (hn =? fvar) eqn: eq_hn_fvar.
+    * destruct hv eqn: eq_hv.
+      -- apply IH with (n:=n); try assumption.
+      -- rewrite -> eval_asfs2_ho. rewrite -> eval_asfs2_ho.
+         pose proof (IH map' ops n stack H eq_optimize_t) as IHc.
+         pose proof (eq_eval_elem_stack stack t map' ops args IHc) as
+           eq_eval_t_map'.
+         rewrite -> eq_eval_t_map'. reflexivity.
+    * apply IH with (n:=n); try assumption.
+Qed.
+
+Theorem optimize_or_zero_fvar_eq: forall (a1 a2: asfs) (fresh_var: nat)
+  (c: tstack) (ops: opm),
+ops OR = Some (Op true 2 or) ->
+optimize_or_zero_fvar fresh_var a1 = Some a2 ->
+eval_asfs c a1 ops = eval_asfs c a2 ops.
+Proof.
+intros.
+destruct a1 as [h1 maxid1 s1 m1] eqn: eq_a1.
+destruct a2 as [h2 maxid2 s2 m2] eqn: eq_a2.
+simpl in H0.
+destruct (optimize_map_or_zero fresh_var m1) eqn: eq_opt_map;
+  try discriminate.
+injection H0 as Hh1h2 Hmaxid1_2 Hs1s2 Hm1a.
+rewrite -> Hm1a in eq_opt_map.
+pose proof (eq_eval_opt_or_zero m1 m2 ops fresh_var c H eq_opt_map)
+  as Hall_elem_eval_same_m1_m2.
+simpl. rewrite -> Hh1h2. rewrite -> Hs1s2.
+destruct (length c =? h2); try reflexivity.
+apply eq_eval_elem_stack. assumption.
+Qed.
+
+
+Lemma opt_or_zero_same_fvar_in_maps: forall (n: nat)
+  (m1 m2: asfs_map),
+optimize_map_or_zero n m1 = Some m2 ->
+same_fvar_in_maps m1 m2.
+Proof.
+intros n m1. revert n.
+induction m1 as [| h t IH].
+- intros n m2 Hopt. simpl in Hopt. discriminate.
+- intros n m2 Hopt.
+  simpl in Hopt.
+  destruct h as [fvar efvar] eqn: eq_h.
+  destruct (fvar =? n) eqn: eq_fvar_n.
+  + destruct efvar eqn: eq_efvar; try discriminate.
+    destruct opcode eqn: eq_opcode; try discriminate.
+    destruct args as [| arg1 targs1] eqn: eq_args; try discriminate.
+    destruct targs1 as [| arg2 targs2] eqn: eq_args1; try discriminate.
+    destruct targs2 eqn: eq_args2; try discriminate.
+    destruct (stack_val_has_value' arg1 t WZero).
+    * injection Hopt as eq_m2. rewrite <- eq_m2.
+      simpl. split; try reflexivity.
+      apply same_fvar_refl.
+    * destruct (stack_val_has_value' arg2 t WZero); try discriminate.
+      injection Hopt as eq_m2. rewrite <- eq_m2.
+      simpl. split; try reflexivity.
+      apply same_fvar_refl.
+  + destruct (optimize_map_or_zero n t) as [t_opt|] eqn: optimize_t;
+      try discriminate.
+    pose proof (strictly_decreasing_preserv fvar efvar t) 
+      as Hdecr_t.
+    pose proof (IH n t_opt optimize_t).
+    simpl. injection Hopt as eq_m2. rewrite <- eq_m2.
+    split; try reflexivity. assumption.
+Qed.
+
+
+Lemma opt_or_zero_decreasingness_preservation: forall (n: nat)
+  (m1 m2: asfs_map),
+strictly_decreasing_map m1 ->
+optimize_map_or_zero n m1 = Some m2 ->
+strictly_decreasing_map m2.
+Proof.
+intros.
+apply opt_or_zero_same_fvar_in_maps in H0.
+apply same_fvar_in_map_preserves_decreasingness with (m1:=m1);
+  try assumption.
+Qed.
+
+
+Lemma optimize_or_zero_fvar_safe:
+safe_optimization_fvar optimize_or_zero_fvar.
+Proof.
+unfold safe_optimization_fvar. intros.
+split.
+- assert (opmap OR = Some (Op true 2 or)) as Hopmap; try reflexivity.
+  pose proof (optimize_or_zero_fvar_eq a opt_a n c opmap Hopmap H0)
+    as Heq_eval_a_opta.
+  rewrite -> Heq_eval_a_opta in H.
+  rewrite -> H.
+  split; try reflexivity.
+- unfold valid_asfs.
+  destruct opt_a as [hopt maxopt sopt mopt] eqn: eq_opt_a.
+  destruct a as [ha maxa sa ma] eqn: eq_a.
+  simpl in H1. simpl in H0.
+  destruct (optimize_map_or_zero n ma) eqn: optimize_ma; try discriminate.
+  injection H0 as eq_h eq_max eq_stack eq_maps. 
+  rewrite -> eq_maps in optimize_ma.
+  destruct H1 as [Hfreshv Hdecr].
+  rewrite <- eq_max.
+  rewrite <- eq_maps.
+  split.
+  + apply same_fvar_in_map_preserves_fresh_var_gt with (m1:=ma).
+    * assumption.
+    * apply opt_or_zero_same_fvar_in_maps with (n:=n).
+      rewrite -> eq_maps. assumption.
+  + apply opt_or_zero_decreasingness_preservation with (n:=n) (m1:=ma) 
+      (m2:=a0) in Hdecr.
+    * assumption.
+    * rewrite -> eq_maps. assumption.
+Qed.
+
 
 Theorem optimize_or_zero_safe:
 safe_optimization optimize_or_zero.
 Proof.
-Admitted.
+apply optimize_fresh_var_preservation.
+apply optimize_or_zero_fvar_safe.
+Qed.
 
 
 
